Hybrid/Examples/SMC/Lemmas.lean
@@ -1,5 +1,6 @@
 import Hybrid.Examples.SMC.Axioms
 import Hybrid.Proof
+import Hybrid.Proof.NewProofs
 
 open SMC
 
@@ -53,37 +54,44 @@ def aleq  (n1 n2 : SMCForm Nat)
 def dplus : SMCProof _
   (c(a1 + a2) ←→ c(a1) ; c(a2) ; plus) := .ax ⟨_, .intro .DPlus⟩
 
-end Axioms
-
-section Propagation
-
-def propagateSeq {s1 s2 : SMCForm Stmt} (h : SMCProof _ (φ ⟶ [c(s1) ; c(s2)] cfg)) : SMCProof _ (φ ⟶ [c(s1 ; s2)] cfg) := by sorry
-
-def assgnVar (s : SMCForm Var) (x : SMCForm Var):
-  SMCProof _  (⟨vs, mem⟩ ⟶ [c(x)] ⟨v ⬝ vs, mem⟩) →
-  SMCProof _  (⟨vs, mem⟩ ⟶ [c(s ::= x)] ⟨vs, set(mem, s, v)⟩) := by
-    sorry
-
 def bubble3Mem (neq1 : x ≠ y) (neq2 : x ≠ z) :
   SMCProof _
     (set(set(set(mem, x, vx), y, vy), z, vz) ←→ set(set(set(mem, y, vy), z, vz), x, vx)) :=
       Proof.ax ⟨_, Nonempty.intro (.ABubble3Mem neq1 neq2)⟩
 
-def propagateMemL {mem1 mem2 : SMCForm Mem}
-  (h1 : SMCProof _ (mem1 ←→ mem2))
-  (h2 : SMCProof _ (⟨vs, mem2⟩ ⟶ [pgm] cfg)) : SMCProof _ (⟨vs, mem1⟩ ⟶ [pgm] cfg) := by sorry
+def nleq {n1 n2 : ℕ}: SMCProof _
+  ((n1 <=Nat n2) ←→ n1.ble n2) := .ax ⟨_, .intro .NLeq⟩
 
-def propagateMemR {mem1 mem2 : SMCForm Mem}
-  (h1 : SMCProof _ (mem1 ←→ mem2))
-  (h2 : SMCProof _ (cfg ⟶ [pgm] ⟨vs, mem2⟩)) : SMCProof _ (cfg ⟶ [pgm] ⟨vs, mem1⟩) := by sorry
+end Axioms
 
-def propagateStackL {vs1 vs2 : SMCForm ValStack}
-  (h1 : SMCProof _ (vs1 ←→ vs2))
-  (h2 : SMCProof _ (⟨vs2, mem⟩ ⟶ [pgm] cfg)) : SMCProof _ (⟨vs1, mem⟩ ⟶ [pgm] cfg) := by sorry
+section Propagation
 
-def propagateDAsgn {v : SMCForm AExp} (h : SMCProof _ (φ ⟶ [c(v); asgn(s)] cfg)) : SMCProof _ (φ ⟶ [c(s ::= v)] cfg) := by
-  simp [Evaluable.ctrlStackEval] at h ⊢
-  have C : (∼(c(v); asgn(s))).Context (∼(c(v); asgn(s)), cfg) := .head
+def propagateNLeq {n1 n2 : ℕ} (h : n1.ble n2):
+    SMCProof _ (n1 <=Nat n2) := by
+  have l1 : SMCProof Bool ((n1 <=Nat n2) ←→ n1.ble n2) := nleq
+  rw [h] at l1
+  apply mp (mp conj_elimR_proof l1)
+  exact ax ⟨_, .intro .ATrue⟩
+
+def propagateSeq {s1 s2 : SMCForm Stmt}
+    (h : SMCProof _ (φ ⟶ [c(s1) ; c(s2)] cfg)) :
+  SMCProof _ (φ ⟶ [c(s1 ; s2)] cfg) := by
+  have propagateNeg : SMCProof _ ((∼c(s1 ; s2)) ←→ ∼(c(s1); c(s2))) := simpNeg <| .ax ⟨_, .intro .CStmtAx⟩
+  have propagateSigma := @simpDualAppl
+            String _ SMC CtrlStack
+            _ _ _
+            propagateNeg
+            _ _
+            (∼(c(s1 ; s2)), cfg)
+            _
+            PDLOp .head
+  have propagateImplL : SMCProof _ ((φ ⟶ _) ←→ (φ ⟶ _)) := simpImplL propagateSigma
+  apply mp _ h
+  apply mp conj_elimR_proof
+  exact propagateImplL
+
+def propagateDAsgn {v : SMCForm AExp} (h : SMCProof _ (φ ⟶ [c(v); asgn(s)] cfg)) :
+    SMCProof _ (φ ⟶ [c(s ::= v)] cfg) := by
   have propagateNeg : SMCProof _ ((∼c(s ::= v)) ←→ ∼(c(v); asgn(s))) := simpNeg dasgn
   have propagateSigma := @simpDualAppl
             String _ SMC CtrlStack
@@ -100,36 +108,131 @@ def propagateDAsgn {v : SMCForm AExp} (h : SMCProof _ (φ ⟶ [c(v); asgn(s)] cf
 
 def propagateDIf {bexp : SMCForm BExp}
     (h : SMCProof _ (φ ⟶ [c(bexp) ; ((true : CtNoms Val) ? ; c(s1)) ∪ ((false : CtNoms Val) ? ; c(s2))] ψ)) :
-  SMCProof _ (φ ⟶ [c(if bexp then s1 else s2 endif)] ψ) := sorry
+  SMCProof _ (φ ⟶ [c(if bexp then s1 else s2 endif)] ψ) := by
+  let ctrlStack := c(bexp) ; ((true : CtNoms Val) ? ; c(s1)) ∪ ((false : CtNoms Val) ? ; c(s2))
+  have C : (∼(ctrlStack)).Context (∼(ctrlStack), ψ) := .head
+  have propagateNeg : SMCProof _ ((∼ctrlStack) ←→ ∼(c(if bexp then s1 else s2 endif))) := simpNeg <| .ax ⟨_, .intro .DIf⟩
+  have propagateSigma := @simpDualAppl
+            String _ SMC CtrlStack
+            _ _ _
+            propagateNeg
+            _ _
+            (∼(ctrlStack), ψ)
+            _
+            PDLOp .head
+  have propagateImplL : SMCProof _ ((φ ⟶ _) ←→ (φ ⟶ _)) := simpImplL propagateSigma
+  apply mp _ h
+  apply mp conj_elimL_proof
+  exact propagateImplL
+
+def propagateDLeq {a1 a2 : SMCForm AExp}
+  (h : SMCProof _ (φ ⟶ [c(a1) ; c(a2) ; leq] ψ)):
+  SMCProof _ (φ ⟶ [c(a1 <= a2)] ψ) := by
+  let ctrlStack := c(a1) ; c(a2) ; leq
+  have C : (∼(ctrlStack)).Context (∼(ctrlStack), ψ) := .head
+  have propagateNeg : SMCProof _ ((∼(c(a1 <= a2)) ←→ (∼(c(a1) ; c(a2) ; leq)))) := simpNeg dleq
+  have propagateSigma := @simpDualAppl
+            String _ SMC CtrlStack
+            _ _ _
+            propagateNeg
+            _ _
+            (∼(c(a1 <= a2)), ψ)
+            _
+            PDLOp .head
+  have propagateImplL : SMCProof _ ((φ ⟶ _) ←→ (φ ⟶ _)) := simpImplL propagateSigma
+  apply mp _ h
+  apply mp conj_elimR_proof
+  exact propagateImplL
+
+def propagateMemL {mem1 mem2 : SMCForm Mem}
+    (h1 : SMCProof _ (mem1 ←→ mem2))
+    (h2 : SMCProof _ (⟨vs, mem2⟩ ⟶ [pgm] cfg)) : SMCProof _ (⟨vs, mem1⟩ ⟶ [pgm] cfg) := by
+  apply imp_trans_proof _ h2
+  apply mp conj_elimL_proof (simpAppl _ (.tail .refl))
+  exact h1
+
+def propagateStackL {vs1 vs2 : SMCForm ValStack}
+    (h1 : SMCProof _ (vs1 ←→ vs2))
+    (h2 : SMCProof _ (⟨vs2, mem⟩ ⟶ [pgm] cfg)) : SMCProof _ (⟨vs1, mem⟩ ⟶ [pgm] cfg) := by
+  apply imp_trans_proof _ h2
+  apply mp conj_elimL_proof (simpAppl _ .head)
+  exact h1
+
+def propagateStackL' {vs1 vs2 : SMCForm ValStack}
+    (h1 : SMCProof _ (vs1 ⟶ vs2))
+    (h2 : SMCProof _ (⟨vs2, mem⟩ ⟶ [pgm] cfg)) : SMCProof _ (⟨vs1, mem⟩ ⟶ [pgm] cfg) := by
+  apply imp_trans_proof _ h2
+  let C : (vs1).Context (vs1, mem) := .head
+  have : (vs2, mem) = C[vs2] := rfl
+  simp [config, this]
+  apply impAppl
+  exact h1
+
+def propagateMemR {mem1 mem2 : SMCForm Mem}
+    (h1 : SMCProof _ (mem1 ←→ mem2))
+    (h2 : SMCProof _ (cfg ⟶ [pgm] ⟨vs, mem2⟩)) : SMCProof _ (cfg ⟶ [pgm] ⟨vs, mem1⟩) := by
+  apply imp_trans_proof h2
+  let C : (⟨vs, mem2⟩ ⟶ ⟨vs, mem1⟩).Context (∼pgm, ⟨vs, mem2⟩ ⟶ ⟨vs, mem1⟩) := .tail .refl
+  have : (∼pgm, ⟨vs, mem1⟩) = C[⟨vs, mem1⟩] := rfl
+  simp [pdlOp, this]
+  have : (∼pgm, ⟨vs, mem2⟩) = C[⟨vs, mem2⟩] := rfl
+  simp [this]
+  apply mp (k _ _ _ _ C)
+  apply ug (.tail .refl)
+  let C' : mem2.Context (vs, mem2) := .tail .refl
+  have : (vs, mem1) = C'[mem1] := rfl
+  simp [config, this]
+  apply impAppl C'
+  exact mp conj_elimR_proof h1
 
 def propagateACup
     (h1 : SMCProof _ (φ ⟶  [π] γ))
     (h2 : SMCProof _ (φ ⟶ [π'] γ)) :
-  SMCProof _ (φ ⟶ [π ∪ π'] γ) := sorry
-
-def propagateDLeq {a1 a2 : SMCForm AExp}
-  (h : SMCProof _ (φ ⟶ [c(a1) ; c(a2) ; leq] ψ)):
-  SMCProof _ (φ ⟶ [c(a1 <= a2)] ψ) := sorry
+      SMCProof _ (φ ⟶ [π ∪ π'] γ) := by
+  let l1 : SMCProof _ ((([π] γ) ⋀ [π'] γ) ⟶ [π ∪ π'] γ) := mp conj_elimL_proof (ax ⟨_, .intro .ACup⟩)
+  apply imp_trans_proof _ l1
+  apply conj_intro_hyp
+  repeat assumption
 
 def propagateDAdd {n m : ℕ} :
   SMCProof _ (⟨(n + m) ⬝ vs, mem⟩ ⟶ [α] φ)
-  → SMCProof _ (⟨(n +Nat m) ⬝ vs, mem⟩ ⟶ [α] φ) := sorry
+  → SMCProof _ (⟨(n +Nat m) ⬝ vs, mem⟩ ⟶ [α] φ) := by
+  apply propagateStackL'
+  let C : ((n +Nat m):SMCForm Val).Context (((n +Nat m):SMCForm Val), vs) := .head
+  let add : SMCForm Val := n+m
+  have : (add, vs) = C[add] := rfl
+  simp [add] at this
+  simp [stackCons, this]
+  apply impAppl
+  apply mp conj_elimL_proof
+  exact .ax ⟨_, .intro .APlusNat⟩
 
 end Propagation
 
 section Lemmas
 
-def atInv :
-  SMCProof _ (ℋ@ i φ ⟶ [α] ℋ@ i φ) := sorry
-
 def kPgm :
-  SMCProof _ (([α] φ ⟶ ψ) ⟶ ([α] φ) ⟶ ([α] ψ)) := sorry
+  SMCProof _ (([α] φ ⟶ ψ) ⟶ ([α] φ) ⟶ ([α] ψ)) :=
+   k _ _ _ _ (.tail .refl)
 
 def necessPgm :
-  SMCProof _ φ → SMCProof _ ([α] φ) := sorry
+  SMCProof _ φ → SMCProof _ ([α] φ) :=
+    ug (.tail .refl)
+
+def atInv :
+  SMCProof _ (ℋ@ i φ ⟶ [α] ℋ@ i φ) :=
+    backContrapositive (.tail .refl)
 
 def falseNatLeq {n m : ℕ} (h : n.ble m) :
-  SMCProof s (ℋ@ false ((n <=Nat m):SMCForm Val) ⟶ ℋ⊥) := sorry
+  SMCProof s (ℋ@ false ((n <=Nat m):SMCForm Val) ⟶ ℋ⊥) := by
+  apply imp_trans_proof
+  . exact mp conj_elimR_proof (ax ⟨_, .intro .AFalseValEmbed⟩)
+  . apply imp_trans_proof
+    . apply mp conj_elimL_proof
+      exact ax ⟨_, .intro .AFalse⟩
+    . apply mp dni'
+      apply genAt
+      exact propagateNLeq h
 
 end Lemmas
 
@@ -170,6 +273,14 @@ def composition
   have l4 : SMCProof _ (φ₀ ⟶ [α₁][α₂] φ₂) := imp_trans_proof h1 l3
   have l5 := imp_trans_proof l4 aseqR
   exact l5
+
+def assignment (s : SMCForm Var) (x : SMCForm Var):
+  SMCProof _  (⟨vs, mem⟩ ⟶ [c(x)] ⟨v ⬝ vs, mem⟩) →
+  SMCProof _  (⟨vs, mem⟩ ⟶ [c(s ::= x)] ⟨vs, set(mem, s, v)⟩) := by
+  intro h
+  apply propagateDAsgn
+  apply composition h
+  apply aasgn
 
 def conditional {b : SMCForm BExp}
     (h1 : SMCProof _ (φ ⟶ [c(b)] ⟨B ⬝ vs, mem⟩))
@@ -215,9 +326,6 @@ def aplus {n1 n2 : SMCForm Nat} : SMCProof _
 def aplus' {n1 n2 : SMCForm Nat} {v : SMCForm Val} : SMCProof _
     (⟨(n2 ⋀ v) ⬝ n1 ⬝ vs, mem⟩ ⟶ [plus] ⟨(n1 +Nat n2) ⬝ vs, mem⟩) := sorry
 
-def nleq {n1 n2 : ℕ}: SMCProof _
-  ((n1 <=Nat n2) ←→ n1.ble n2) := .ax ⟨_, .intro .NLeq⟩
-
 def aind : SMCProof _
   (γ ⋀ [π*](γ ⟶ [π]γ) ←→ [π*] γ) := .ax ⟨_, .intro .AInd⟩
 
@@ -234,10 +342,6 @@ def propagateDWhile {bexp : SMCForm BExp}
 def propagateDEq {a1 a2 : SMCForm AExp}
   (h : SMCProof _ (φ ⟶ [c(a1) ; c(a2) ; eq] ψ)):
   SMCProof _ (φ ⟶ [c(a1 is a2)] ψ) := sorry
-
-def propagateNLeq {n1 n2 : ℕ}
-    (h : SMCProof _ (φ ⟶ [α] ⟨(n1.ble n2) ⬝ vs, mem⟩)):
-  SMCProof _ (φ ⟶ [α] ⟨(n1 <=Nat n2) ⬝ vs, mem⟩) := sorry
 
 def propagateDPlus
     (h : SMCProof _ (φ ⟶ [c(a1) ; c(a2) ; plus] ψ)):
