Hybrid/Proof/NewProofs.lean
@@ -1,0 +1,50 @@
+import Hybrid.Proof.Equiv
+
+namespace Proof
+
+variable {α : Type u}
+variable [DecidableEq α]
+variable {symbs : Symbols α}
+variable {Λ : AxiomSet symbs}
+
+def negAt :
+    Proof Λ s (ℋ@ i (∼φ) ⟶ ∼(ℋ@ i φ)) := by
+  apply imp_trans_proof
+  . exact mp conj_elimL_proof (selfDual _ _)
+  . apply mp contraposition
+    apply mp (kAt _ _ _)
+    apply genAt
+    exact dni
+
+def negAt' :
+    Proof Λ s (∼(ℋ@ i φ) ⟶ ℋ@ i (∼φ)) := by
+  apply mp contraposition''
+  exact mp conj_elimR_proof (selfDual _ _)
+
+def backContrapositive (C : (@FormL.at α symbs t sᵢ i φ).Context ψ) :
+    Proof Λ s (ℋ@i φ ⟶ ℋ⟨σ⟩ᵈ ψ) := by
+  unfold FormL.applDual
+  apply mp contraposition'
+  apply imp_trans_proof _ negAt
+  have ⟨χ, C', eq, iso, _⟩ := C.to_negAll
+  subst eq
+  apply imp_trans_proof
+  . apply impAppl C' negAt'
+  . apply back
+    apply FormL.subst_to_ctx
+
+def kAt_disj {k : symbs.nominal t} : Proof Λ s (ℋ@ k (φ ⋁ ψ) ⟶ ℋ@ k φ ⋁ ℋ@ k ψ) := by
+  apply imp_trans_proof _ impAsDisj
+  apply imp_com_proof
+  apply imp_trans_proof negAt'
+  apply imp_trans_proof _ (kAt _ _ _)
+  apply mp (kAt _ _ _)
+  apply genAt
+  apply imp_com_proof
+  apply disj_elim_not
+
+def tertium_non_daturAt_proof (k : symbs.nominal t) (φ : Form symbs t) : Proof Λ s (ℋ@ k φ ⋁ ℋ@ k (∼φ)) := by
+  have l1 : Proof Λ _ (φ ⋁ (∼φ)) := tertium_non_datur_proof
+  have l2 := genAt s k l1
+  have l3 := mp kAt_disj l2
+  exact l3
